compcertox/Lifting.v
@@ -1,7 +1,12 @@
 Require Import Relations RelationClasses Relators.
 Require Import List.
 Require Import Coqlib.
-Require Import LanguageInterface_ Events Globalenvs Smallstep_.
+Require Import LanguageInterface_ Events Globalenvs.
+Require Import CategoricalComp.
+Require Import SmallstepLinking_.
+Require Import Smallstep_.
+Require Import Linking.
+Require Import CompCertO.
 
 (* Definitions *)
 Section Lifting.
@@ -64,7 +69,6 @@ Notation "L @ K" := (lifted_semantics K L): lts_scope.
 Notation " 'layer' K " := (Smallstep_.semantics li_null (li_c @ K)) (at level 1).
 
 (* Properties *)
-Require Import CategoricalComp.
 
 Section CAT_COMP_LIFT.
   Variable K: Type.
@@ -104,11 +108,11 @@ Section CAT_COMP_LIFT.
       + eexists. split. apply step2.
         instantiate (1 := (_, _)). econstructor; eauto.
         constructor.
-      + eexists. split. eapply step_push.
+      + eexists. split. eapply CategoricalComp.step_push.
         instantiate (1 := (_, _)). constructor; cbn; eauto.
         instantiate (1 := (_, _)). econstructor; cbn; eauto.
         auto. auto. constructor.
-      + eexists. split. eapply  step_pop.
+      + eexists. split. eapply  CategoricalComp.step_pop.
         instantiate (1 := (_, _)). econstructor; cbn; eauto.
         instantiate (1 := (_, _)). econstructor; cbn; eauto.
         constructor.
@@ -146,10 +150,10 @@ Section CAT_COMP_LIFT.
         apply step2. auto.
       + destruct q, s3. inv H. inv H0. cbn in *. subst.
         eexists (_, _); split; constructor; auto.
-        eapply step_push; eauto.
+        eapply CategoricalComp.step_push; eauto.
       + destruct r, s1'0. inv H. inv H0. cbn in *. subst.
         eexists (_, _); split; constructor; auto.
-        eapply step_pop; eauto.
+        eapply CategoricalComp.step_pop; eauto.
     - apply well_founded_ltof.
       Unshelve. exact tt.
   Qed.
@@ -161,3 +165,394 @@ Section CAT_COMP_LIFT.
   Qed.
 
 End CAT_COMP_LIFT.
+
+Section HCOMP_LIFT.
+  Variable K: Type.
+  Context {li} (L1: Smallstep_.semantics li li)
+          (L2: Smallstep_.semantics li li).
+  Variable (sk: AST.program unit unit).
+
+  Let L := fun b => match b with | true => L1 | false => L2 end.
+  Let LK := fun b => match b with | true => L1@K | false => L2@K end.
+
+  (* if i remains a variable, it won't type check *)
+  Inductive match_cont: list (frame L) -> list (frame LK) -> Prop :=
+  | match_cont_nil: match_cont nil nil
+  | match_cont_t s k cont kcont:
+      match_cont cont kcont ->
+      match_cont (st L true s :: cont) (st LK true (s, k) :: kcont)
+  | match_cont_f s k cont kcont:
+      match_cont cont kcont ->
+      match_cont (st L false s :: cont) (st LK false (s, k) :: kcont).
+
+  Inductive state_match_hcomp: (list (frame L) * K) -> list (frame LK) -> Prop :=
+
+  | state_match_hcomp_t s k cont kcont:
+      match_cont cont kcont ->
+      state_match_hcomp (st L true s :: cont, k) (st LK true (s, k) :: kcont)
+  | state_match_hcomp_f s k cont kcont:
+      match_cont cont kcont ->
+      state_match_hcomp (st L false s :: cont, k) (st LK false (s, k) :: kcont).
+
+  Hint Constructors state_match_hcomp match_cont.
+
+  Lemma lift_horizontal_comp1:
+    (SmallstepLinking_.semantics L sk)@K ≤ SmallstepLinking_.semantics LK sk.
+  Proof.
+    constructor. econstructor. reflexivity. intros i. reflexivity.
+    intros se _ [ ] ? [ ] Hse. instantiate (1 := fun _ _ _ => _). cbn beta.
+    eapply forward_simulation_step with (match_states := state_match_hcomp).
+    - intros [q kq] ? [s ks] [ ] H. inv H. inv H0.
+      cbn in *. subst.
+      destruct i; eexists.
+      + split; eauto. constructor. firstorder. now constructor.
+      + split; eauto. constructor. firstorder. now constructor.
+    - intros [s1 ks1] s2 [r ks] Hs H. inv H. inv H0.
+      inv Hs; cbn in *; subst.
+      + inv H2. SmallstepLinking_.subst_dep. inv H5.
+        eexists; split; eauto. repeat constructor. auto.
+      + inv H2. SmallstepLinking_.subst_dep. inv H5.
+        eexists; split; eauto. repeat constructor. auto.
+    - intros [s1 ks1] s2 [q kq] Hs H. inv H. inv H0.
+      inv Hs; cbn in *; subst.
+      + inv H3. SmallstepLinking_.subst_dep.
+        eexists _, (_, _). repeat apply conj; auto.
+        constructor.
+        * constructor; cbn; auto.
+        * intros j. specialize (H2 j). intros Hvq. apply H2.
+          destruct j; firstorder.
+        * intros [r1 kr1] [r2 kr2] [s1' ks1'] <- Haft.
+          inv Haft. inv H0. cbn in *. SmallstepLinking_.subst_dep.
+          eexists; split; eauto. constructor. now constructor.
+      + inv H3. SmallstepLinking_.subst_dep.
+        eexists _, (_, _). repeat apply conj; auto.
+        constructor.
+        * constructor; cbn; auto.
+        * intros j. specialize (H2 j). intros Hvq. apply H2.
+          destruct j; firstorder.
+        * intros [r1 kr1] [r2 kr2] [s1' ks1'] <- Haft.
+          inv Haft. inv H0. cbn in *. SmallstepLinking_.subst_dep.
+          eexists; split; eauto. constructor. now constructor.
+    - intros [s1 ks1] t [s1' ks1'] Hstep s2 Hs. inv Hstep.
+      inv H; inv Hs; SmallstepLinking_.subst_dep.
+      + eexists; split; eauto.
+        apply step_internal. constructor; auto.
+      + eexists; split; eauto.
+        apply step_internal. constructor; auto.
+      + destruct j; eexists; split.
+        * eapply step_push with (q0 := (_, _)) (j := true) (s'0 := (_, _));
+            try split; cbn; eauto; try firstorder; auto.
+        * auto.
+        * eapply step_push with (q0 := (_, _)) (j := false) (s'0 := (_, _));
+            try split; cbn; eauto; try firstorder; auto.
+        * auto.
+      + destruct j; eexists; split.
+        * eapply step_push with (q0 := (_, _)) (j := true) (s'0 := (_, _));
+            try split; cbn; eauto; try firstorder; auto.
+        * auto.
+        * eapply step_push with (q0 := (_, _)) (j := false) (s'0 := (_, _));
+            try split; cbn; eauto; try firstorder; auto.
+        * auto.
+      + inv H6; SmallstepLinking_.subst_dep; eexists; split.
+        * eapply step_pop with (r0 := (_, _)) (s'0 := (_, _));
+            constructor; cbn; eauto.
+        * auto.
+        * eapply step_pop with (r0 := (_, _)) (s'0 := (_, _));
+            constructor; cbn; eauto.
+        * auto.
+      + inv H6; SmallstepLinking_.subst_dep; eexists; split.
+        * eapply step_pop with (r0 := (_, _)) (s'0 := (_, _));
+            constructor; cbn; eauto.
+        * auto.
+        * eapply step_pop with (r0 := (_, _)) (s'0 := (_, _));
+            constructor; cbn; eauto.
+        * auto.
+    - apply well_founded_ltof.
+      Unshelve. exact tt. exact tt.
+  Qed.
+
+  (* Goal forall s0 s k, *)
+  (*     state_match_hcomp (st L true s0 :: nil, k) (st LK true (s, k) :: nil) *)
+  (*     -> s = s0. *)
+  (* Proof. *)
+  (*   intros. remember (st LK true (s, k)) as ss. *)
+  (*   inversion H. subst. *)
+  (*   unfold LK in *. *)
+  (* Admitted. *)
+
+  (* Goal forall s0 s, (st L true s) = (st L true s0) -> s0 = s. *)
+  (*   intros. inversion H. *)
+  (* Admitted. *)
+
+  Lemma foo: forall s0 s, (st LK true s0) = (st LK true s) -> s0 = s.
+  Proof.
+    intros. inversion H.
+    SmallstepLinking_.subst_dep. reflexivity.
+  Qed.
+
+  Lemma foo': forall s0 s, (st LK false s0) = (st LK false s) -> s0 = s.
+  Proof.
+    intros. inversion H.
+    SmallstepLinking_.subst_dep. reflexivity.
+  Qed.
+
+  Lemma destruct_ms1 s k cont' s' k':
+    state_match_hcomp (s, k) (st LK true (s', k') :: cont') ->
+    exists cont, s = st L true s' :: cont /\ match_cont cont cont' /\ k = k'.
+  Proof.
+    intros. remember (st LK true (s', k') :: cont') as ss. inv H.
+    - remember (st LK true (s0, k)) as sst.
+      remember (st LK true (s', k')) as st'.
+      inv H1.
+      (* remember (s', k') as sk'. *)
+      (* remember (s0, k) as sk0. *)
+      apply foo in H0. inv H0. eexists; repeat apply conj; eauto.
+    - remember (st LK false (s0, k)) as sst.
+      remember (st LK true (s', k')) as st'.
+      inv H1. inv H0.
+  Qed.
+
+  Lemma destruct_ms2 s k cont' s' k':
+    state_match_hcomp (s, k) (st LK false (s', k') :: cont') ->
+    exists cont, s = st L false s' :: cont /\ match_cont cont cont' /\ k = k'.
+  Proof.
+    intros. remember (st LK false (s', k') :: cont') as ss. inv H.
+    - remember (st LK true (s0, k)) as sst.
+      remember (st LK false (s', k')) as st'.
+      inv H1. inv H0.
+    - remember (st LK false (s0, k)) as sst.
+      remember (st LK false (s', k')) as st'.
+      inv H1.
+      apply foo' in H0. inv H0. eexists; repeat apply conj; eauto.
+  Qed.
+
+  Lemma destruct_mcont1 x s k cont:
+    match_cont x (st LK true (s, k) :: cont) ->
+    exists kk, x = st L true s :: kk  /\ match_cont kk cont.
+  Proof.
+    intros. remember (st LK true (s, k) :: cont) as ss. inv H.
+    - inv H1.
+    - remember (st LK true (s0, k0)) as st0.
+      remember (st LK true (s, k)) as skk.
+      inv H2. apply foo in H1. inv H1.
+      eexists; split; eauto.
+    - inv H2.
+  Qed.
+
+  Lemma destruct_mcont2 x s k cont:
+    match_cont x (st LK false (s, k) :: cont) ->
+    exists kk, x = st L false s :: kk /\ match_cont kk cont.
+  Proof.
+    intros. remember (st LK false (s, k) :: cont) as ss. inv H.
+    - inv H1.
+    - inv H2.
+    - remember (st LK false (s0, k0)) as st0.
+      remember (st LK false (s, k)) as skk.
+      inv H2. apply foo' in H1. inv H1.
+      eexists; split; eauto.
+  Qed.
+
+  Lemma lift_horizontal_comp2:
+    SmallstepLinking_.semantics LK sk ≤ (SmallstepLinking_.semantics L sk)@K.
+  Proof.
+    constructor. econstructor. reflexivity. intros i. reflexivity.
+    intros se _ [ ] ? [ ] Hse. instantiate (1 := fun _ _ _ => _). cbn beta.
+    eapply forward_simulation_step
+      with (match_states := fun s1 s2 => state_match_hcomp s2 s1).
+    - intros [q1 kq1] [? ?] s1 [ ] H. inv H.
+      destruct i; destruct s; eexists (_, _); split; eauto.
+      * inv H1. cbn in *; subst. constructor; auto.
+        constructor; cbn; firstorder.
+      * inv H1. cbn in *; subst. constructor; auto.
+        constructor; cbn; firstorder.
+    - intros s1 [s2 ks2] [r kr] Hs H. inv H.
+      destruct i; destruct s; inv H0.
+      + apply destruct_ms1 in Hs as (?&?&?&?).
+        cbn in *. inv H2.
+        eexists; split; repeat constructor; auto.
+      + apply destruct_ms2 in Hs as (?&?&?&?).
+        cbn in *. inv H2.
+        eexists; split; repeat constructor; auto.
+    - intros s1 [s2 ks2] [q kq] Hs H. inv H.
+      destruct i; destruct s; inv H0.
+      + apply destruct_ms1 in Hs as (?&?&?&?).
+        cbn in *; subst.
+        eexists tt, (_, _). repeat apply conj; try constructor; cbn; auto.
+        * intros j. specialize (H1 j). destruct j; firstorder.
+        * intros [r1 kr1] [r2 kr2] s1' <- Haft.
+          inv Haft. SmallstepLinking_.subst_dep. inv H7.
+          destruct s'. cbn in *; subst.
+          eexists (_, _); split; eauto. repeat constructor. apply H0.
+      + apply destruct_ms2 in Hs as (?&?&?&?).
+        cbn in *; subst.
+        eexists tt, (_, _). repeat apply conj; try constructor; cbn; auto.
+        * intros j. specialize (H1 j). destruct j; firstorder.
+        * intros [r1 kr1] [r2 kr2] s1' <- Haft.
+          inv Haft. SmallstepLinking_.subst_dep. inv H7.
+          destruct s'. cbn in *; subst.
+          eexists (_, _); split; eauto. repeat constructor. apply H0.
+    - intros s1 t s1' Hstep [s2 ks2] Hs.
+      inv Hstep; destruct i; destruct s.
+      + destruct s'. inv H.
+        apply destruct_ms1 in Hs as (?&?&?&?). subst.
+        eexists (_, _); split; eauto.
+        constructor; auto.
+        eapply step_internal; auto.
+      + destruct s'. inv H.
+        apply destruct_ms2 in Hs as (?&?&?&?). subst.
+        eexists (_, _); split; eauto.
+        constructor; auto.
+        eapply step_internal; auto.
+      + destruct q. inv H.
+        apply destruct_ms1 in Hs as (?&?&?&?). cbn in *; subst.
+        destruct j; destruct s'; inv H1.
+        * eexists (_, _); repeat apply conj; eauto.
+          eapply step_push; eauto.
+        * eexists (_, _); repeat apply conj; eauto.
+          eapply step_push; eauto.
+      + destruct q. inv H.
+        apply destruct_ms2 in Hs as (?&?&?&?). cbn in *; subst.
+        destruct j; destruct s'; inv H1.
+        * eexists (_, _); repeat apply conj; eauto.
+          eapply step_push; eauto.
+        * eexists (_, _); repeat apply conj; eauto.
+          eapply step_push; eauto.
+      + destruct r. inv H. cbn in *; subst.
+        apply destruct_ms1 in Hs as (?&?&?&?).
+        destruct j; destruct s'; destruct sk0; destruct H0; cbn in *; subst.
+        * apply destruct_mcont1 in H2 as (?&?&?). subst.
+          eexists (_, _); repeat apply conj; eauto.
+          eapply step_pop; eauto.
+        * apply destruct_mcont2 in H2 as (?&?&?). subst.
+          eexists (_, _); repeat apply conj; eauto.
+          eapply step_pop; eauto.
+      + destruct r. inv H. cbn in *; subst.
+        apply destruct_ms2 in Hs as (?&?&?&?).
+        destruct j; destruct s'; destruct sk0; destruct H0; cbn in *; subst.
+        * apply destruct_mcont1 in H2 as (?&?&?). subst.
+          eexists (_, _); repeat apply conj; eauto.
+          eapply step_pop; eauto.
+        * apply destruct_mcont2 in H2 as (?&?&?). subst.
+          eexists (_, _); repeat apply conj; eauto.
+          eapply step_pop; eauto.
+    - apply well_founded_ltof.
+  Qed.
+
+  Lemma lift_horizontal_comp:
+    (SmallstepLinking_.semantics L sk)@K ≡ SmallstepLinking_.semantics LK sk.
+  Proof.
+    split; [ exact lift_horizontal_comp1 | exact lift_horizontal_comp2 ].
+  Qed.
+End HCOMP_LIFT.
+
+(* TODO: move this to lifting.v *)
+Lemma lifting_step_star {liA liB K} (L: Smallstep_.semantics liA liB) se qset s1 t s2 k:
+  Star (L se) qset s1 t s2 ->
+  Star(lifted_lts K (L se)) qset (s1, k) t (s2, k).
+Proof.
+  induction 1; [eapply star_refl | eapply star_step]; eauto.
+  constructor; auto.
+Qed.
+
+Lemma lifting_step_plus {liA liB K} (L: Smallstep_.semantics liA liB) se qset s1 t s2 k:
+  Plus (L se) qset s1 t s2 ->
+  Plus (lifted_lts K (L se)) qset (s1, k) t (s2, k).
+Proof.
+  destruct 1; econstructor; eauto using lifting_step_star.
+  split; eauto.
+Qed.
+
+Lemma lifting_simulation {K li1 li2} {L1 L2: Smallstep_.semantics li1 li2}:
+  L1 ≤ L2 -> L1 @ K ≤ L2 @ K.
+Proof.
+  intros [H]. constructor.
+  eapply Forward_simulation with
+      (fsim_order H)
+      (fun se1 se2 w i '(s1, k1) '(s2, k2) =>
+         fsim_match_states H se1 se2 w i s1 s2 /\ k1 = k2).
+  - apply (fsim_skel H).
+  - intros i. apply (fsim_footprint H).
+  - destruct H as [? ? ? ? ? Hf ?]. cbn. clear -Hf.
+    intros se1 se2 [ ] qset Hse Hse'.
+    specialize (Hf se1 se2 tt qset Hse Hse'). subst.
+    econstructor.
+    + intros [q kq] ? [s1 ks] [ ] Hi. inv Hi. cbn in *; subst.
+      exploit (fsim_match_initial_states Hf); eauto. econstructor.
+      intros (? & ? & ? & ?). eexists _, (_, _).
+      repeat apply conj; cbn; eauto.
+    + intros i [s1 ks1] [s2 ks2] [r kr] [Hs Hk] Hi.
+      inv Hi. cbn in *; subst.
+      exploit (fsim_match_final_states Hf); eauto.
+      intros (? & ? & ?). inv H1.
+      eexists (_, _). repeat apply conj; cbn; eauto.
+    + intros i [s1 ks1] [s2 ks2] [q1 kq1] [Hs Hk] Hi.
+      inv Hi. cbn in *; subst.
+      exploit (fsim_match_external Hf); eauto.
+      intros (? & ? & ? & Hq & ? & Hx). inv Hq.
+      eexists tt, (_, _). repeat apply conj; cbn; eauto.
+      intros [r kr] [? ?] [s1' Hs1'] <- Ha. inv Ha.
+      cbn in *; subst. exploit Hx; eauto.
+      intros (? & ? & ? & ?). eexists _, (_, _).
+      repeat apply conj; cbn; eauto.
+    + intros [s1 ks1] t [s1' ks1'] Hstep i [s2 ks2] [Hs Hk].
+      inv Hstep. exploit (fsim_simulation Hf); eauto.
+      intros (? & ? & Hx & ?). destruct Hx.
+      * eexists _, (_, _); repeat apply conj; eauto.
+        left. apply lifting_step_plus; auto.
+      * eexists _, (_, _); repeat apply conj; eauto.
+        right. destruct H1. split; eauto using lifting_step_star.
+  - apply fsim_order_wf.
+Qed.
+
+Definition skel_extend {liA liB} (L: Smallstep_.semantics liA liB) sk :=
+  {|
+  activate se := L se;
+  skel := sk;
+  footprint := footprint L;
+  |}.
+
+(* Lifting a code skeleton *)
+Section SKEL.
+  Context {liA1 liB1 liA2 liB2}
+          {cc1: callconv liA1 liA2}
+          {cc2: callconv liB1 liB2}
+          {L1: Smallstep_.semantics liA1 liB1}
+          {L2: Smallstep_.semantics liA2 liB2}
+          (HL: forward_simulation cc1 cc2 L1 L2).
+  Variable (sk: AST.program unit unit).
+  Hypothesis Hsk: linkorder (skel L1) sk.
+
+  Lemma skel_extend_fsim:
+    forward_simulation cc1 cc2 (skel_extend L1 sk) (skel_extend L2 sk).
+  Proof.
+    unfold skel_extend. destruct HL.
+    constructor. econstructor. reflexivity.
+    - intros; cbn. eapply fsim_footprint. apply X.
+    - intros. exploit (fsim_lts X); eauto. cbn in *.
+      eapply Genv.valid_for_linkorder; eauto.
+    - apply (fsim_order_wf X).
+  Qed.
+End SKEL.
+
+Section SKEL_EXT_LIFT.
+  Context {K1 K2: Type}
+          {liA1 liB1 liA2 liB2: language_interface}
+          {cc1: callconv (liA1@K1) (liA2@K2)}
+          {cc2: callconv (liB1@K1) (liB2@K2)}
+          (L1: Smallstep_.semantics liA1 liB1)
+          (L2: Smallstep_.semantics liA2 liB2).
+  Hypothesis HL: forward_simulation cc1 cc2 (L1@K1) (L2@K2).
+  Variable (sk: AST.program unit unit).
+  Hypothesis Hsk: linkorder (skel L1) sk.
+  Lemma lift_skel_extend:
+    forward_simulation cc1 cc2 (skel_extend L1 sk @ K1)
+                       (skel_extend L2 sk @ K2).
+  Proof.
+    destruct HL as [H]. constructor. econstructor.
+    - reflexivity.
+    - apply (fsim_footprint H).
+    - intros. apply (fsim_lts H); auto.
+      eapply Genv.valid_for_linkorder; eauto.
+    - apply (fsim_order_wf H).
+  Qed.
+End SKEL_EXT_LIFT.
