compcertox/CompCertO.v
@@ -1,0 +1,120 @@
+(* This file contains definitions that will be moved to CompCertO later *)
+
+Require Import Relations RelationClasses Relators.
+Require Import List Maps.
+Require Import Coqlib.
+Require Import CallconvAlgebra_.
+Require Import LanguageInterface_ Events Globalenvs Smallstep_ CategoricalComp FlatComp.
+Require Import Memory Values.
+Require Import Linking.
+
+(* TODO: move this to compcert *)
+Global Instance fsim_transitive {li1 li2: language_interface}:
+  Transitive (forward_simulation (@cc_id li1) (@cc_id li2)).
+Proof.
+  intros L1 L2 L3 HL1 HL2.
+  eapply open_fsim_ccref. apply cc_compose_id_left.
+  unfold flip. apply cc_compose_id_left.
+  eapply compose_forward_simulations; eauto.
+Qed.
+
+
+Section HCOMP_FSIM.
+
+  Context {li1 li2} (cc: callconv li1 li2)
+          (L1a L1b: Smallstep_.semantics li1 li1)
+          (L2a L2b: Smallstep_.semantics li2 li2).
+  Hypothesis (HL1: forward_simulation cc cc L1a L2a)
+             (HL2: forward_simulation cc cc L1b L2b).
+  Let L1 := fun b => match b with | true => L1a | false => L1b end.
+  Let L2 := fun b => match b with | true => L2a | false => L2b end.
+
+  Variable (sk: AST.program unit unit).
+  Hypothesis (Hsk1: linkorder (skel L1a) sk)
+             (Hsk2: linkorder (skel L1b) sk).
+
+  Lemma horizontal_compose_simulation':
+    forward_simulation cc cc (SmallstepLinking_.semantics L1 sk)
+                       (SmallstepLinking_.semantics L2 sk).
+  Proof.
+    destruct HL1 as [Ha]. destruct HL2 as [Hb].
+    assert (HL: forall i, fsim_components cc cc (L1 i) (L2 i)) by (intros [|]; auto).
+    constructor.
+    eapply Forward_simulation with
+        (SmallstepLinking_.order cc L1 L2 HL)
+        (SmallstepLinking_.match_states cc L1 L2 HL).
+    - reflexivity.
+    - intros i. cbn. destruct Ha, Hb.
+      rewrite fsim_footprint, fsim_footprint0. reflexivity.
+    - intros se1 se2 w qset Hse Hse1.
+      eapply SmallstepLinking_.semantics_simulation; eauto.
+      intros [|]; cbn; eapply Genv.valid_for_linkorder; eauto.
+    - clear - HL. intros [i x].
+      induction (fsim_order_wf (HL i) x) as [x Hx IHx].
+      constructor. intros z Hxz. inv Hxz; SmallstepLinking_.subst_dep. eauto.
+  Qed.
+End HCOMP_FSIM.
+
+Section COMP_FSIM.
+
+  Context {liA1 liA2 liB1 liB2 liC1 liC2}
+          {cc1: callconv liA1 liA2}
+          {cc2: callconv liB1 liB2}
+          {cc3: callconv liC1 liC2}
+          (L1a: Smallstep_.semantics liB1 liC1)
+          (L2a: Smallstep_.semantics liB2 liC2)
+          (L1b: Smallstep_.semantics liA1 liB1)
+          (L2b: Smallstep_.semantics liA2 liB2).
+  Hypothesis (HL1: forward_simulation cc2 cc3 L1a L2a)
+             (HL2: forward_simulation cc1 cc2 L1b L2b).
+
+  Variable (sk: AST.program unit unit).
+  Hypothesis (Hsk1: linkorder (skel L1a) sk)
+             (Hsk2: linkorder (skel L1b) sk).
+
+  Lemma categorical_compose_simulation':
+    forward_simulation cc1 cc3 (comp_semantics' L1a L1b sk)
+                       (comp_semantics' L2a L2b sk).
+  Proof.
+    destruct HL1 as [Ha]. destruct HL2 as [Hb].
+    constructor.
+    eapply Forward_simulation
+      with (CategoricalComp.order cc1 cc2 cc3 L1a L1b L2a L2b Ha Hb)
+           (CategoricalComp.match_states cc1 cc2 cc3 L1a L1b L2a L2b Ha Hb).
+    - cbn. destruct Ha, Hb. congruence.
+    - cbn. intros i. destruct Ha, Hb.
+      rewrite fsim_footprint, fsim_footprint0. reflexivity.
+    - intros se1 se2 w qset Hse Hse1.
+      eapply CategoricalComp.semantics_simulation; eauto.
+      eapply Genv.valid_for_linkorder. apply Hsk1. auto.
+      eapply Genv.valid_for_linkorder. apply Hsk2. auto.
+    - clear - Ha Hb. intros [|].
+      + induction (fsim_order_wf Ha f). constructor.
+        intros. inv H1. apply H0. auto.
+      + induction (fsim_order_wf Hb f0). constructor.
+        intros. inv H1. apply H0. auto.
+  Qed.
+
+End COMP_FSIM.
+
+Section HCOMP_ASSOC.
+
+  Context {li} (L1 L2 L3: Smallstep_.semantics li li).
+  Variable (sk: AST.program unit unit).
+  Let L := fun b => match b with
+                 | true => SmallstepLinking_.semantics
+                            (fun b => match b with | true => L1 | false => L2 end) sk
+                 | false => L3
+                 end.
+  Let L' := fun b => match b with
+                  | true => L1
+                  | false => SmallstepLinking_.semantics
+                              (fun b => match b with | true => L2 | false => L3 end) sk
+                  end.
+
+  Lemma horizontal_compose_associativity:
+    SmallstepLinking_.semantics L sk ≤ SmallstepLinking_.semantics L' sk.
+  Proof.
+  Admitted.
+
+End HCOMP_ASSOC.
